update dependencies, bitvector library and refactor bitvector automation

theories/bitvector.v
@@ -4,134 +4,6 @@ From stdpp Require Import options.
 
 Local Open Scope Z_scope.
 
-Lemma Z_bounded_iff_bits_nonneg k n :
-  0 ≤ k → 0 ≤ n →
-  n < 2^k ↔ ∀ l, k ≤ l → Z.testbit n l = false.
-Proof.
-  intros.
-  destruct (decide (n = 0)) as [->|].
-  - setoid_rewrite Z.bits_0. split; [done|]. intros. by apply Z.pow_pos_nonneg.
-  - split.
-    + intros Hb%Z.log2_lt_pow2 l Hl; [| lia]. apply Z.bits_above_log2; lia.
-    + intros Hl.
-      destruct (decide (n < 2^k)); [done|].
-      assert (Z.testbit n (Z.log2 n) = false) as Hbit.
-      { apply Hl, Z.log2_le_pow2; lia. }
-      rewrite Z.bit_log2 in Hbit; [done| lia].
-Qed.
-
-Lemma Z_bounded_iff_bits_nonneg' k n :
-  0 ≤ k → 0 ≤ n →
-  0 ≤ n < 2^k ↔ ∀ l, k ≤ l → Z.testbit n l = false.
-Proof.
-  intros ??. split.
-  - intros ?. apply Z_bounded_iff_bits_nonneg; lia.
-  - intros ?%Z_bounded_iff_bits_nonneg; lia.
-Qed.
-
-Tactic Notation "learn_hyp" constr(p) "as" ident(H') :=
-  let P := type of p in
-  match goal with
-  | H : P |- _ => fail 1
-  | _ => pose proof p as H'
-  end.
-Tactic Notation "learn_hyp" constr(p) :=
-  let H := fresh in learn_hyp p as H.
-
-Lemma Zmul_assoc_comm n2 n1 n3 : n1 * n2 * n3 = n1 * n3 * n2.
-Proof. lia. Qed.
-
-Lemma Zpow_2_mul a : a ^ 2 = a * a.
-Proof. lia. Qed.
-
-Fixpoint Z_to_little (m : nat) (n : Z) (z : Z) : list Z :=
-  match m with
-  | O => []
-  | S m' => Z.land z (Z.ones n) :: Z_to_little m' n (z ≫ n)
-  end.
-
-Fixpoint Z_of_little (n : Z) (bs : list Z) : Z :=
-  match bs with
-  | [] => 0
-  | b :: bs' => Z.lor (Z_of_little n bs' ≪ n) b
-  end.
-
-Lemma Z_ones_spec n m:
-  0 ≤ m → 0 ≤ n →
-  Z.testbit (Z.ones n) m = if decide (m < n) then true else false.
-Proof. intros. case_decide; [ by rewrite Z.ones_spec_low by lia | by rewrite Z.ones_spec_high by lia ]. Qed.
-
-Lemma Z_to_of_little m n bs:
-  m = length bs → 0 ≤ n →
-  Forall (λ b, 0 ≤ b < 2 ^ n) bs →
-  Z_to_little m n (Z_of_little n bs) = bs.
-Proof.
-  intros -> ? Hall. induction Hall as [|b bs ? ? IH]; [done|]; csimpl.
-  f_equal.
-  - apply Z.bits_inj_iff'. intros n' ?.
-    rewrite !Z.land_spec, Z.lor_spec, Z_ones_spec by lia.
-    case_decide.
-    + rewrite andb_true_r, Z.shiftl_spec_low by lia. done.
-    + rewrite !andb_false_r by lia.
-      symmetry. eapply (Z_bounded_iff_bits_nonneg n); lia.
-  - rewrite <-IH at 3. f_equal.
-    apply Z.bits_inj_iff'. intros n' ?.
-    rewrite Z.shiftr_spec, Z.lor_spec, Z.shiftl_spec by lia.
-    assert (Z.testbit b (n' + n) = false) as ->. {
-      eapply (Z_bounded_iff_bits_nonneg n); lia.
-    }
-    rewrite orb_false_r. f_equal. lia.
-Qed.
-
-Lemma Z_of_to_little m n z:
-  0 ≤ n →
-  Z_of_little n (Z_to_little m n z) = z `mod` 2 ^ (m * n).
-Proof.
-  intros. rewrite <-Z.land_ones by nia.
-  revert z. induction m as [|m IH]; simpl. { intros. Z.bitwise. by rewrite andb_false_r. }
-  intros z. rewrite IH.
-  apply Z.bits_inj_iff'. intros n' ?.
-  rewrite Z.land_spec, Z.lor_spec, Z.shiftl_spec, !Z.land_spec by lia.
-  rewrite (Z_ones_spec n n') by lia. case_decide.
-  - rewrite andb_true_r. rewrite Z.testbit_neg_r by lia. simpl.
-    rewrite Z_ones_spec by nia. case_decide; [ by rewrite andb_true_r| nia].
-  - rewrite andb_false_r, orb_false_r.
-    rewrite Z.shiftr_spec by lia. f_equal. { f_equal. lia. }
-    rewrite !Z_ones_spec by nia. repeat case_decide; try done; nia.
-Qed.
-
-Lemma Z_to_little_bound m n z:
-  0 ≤ n →
-  Forall (λ b, 0 ≤ b < 2 ^ n) (Z_to_little m n z).
-Proof.
-  intros ?. revert z. induction m as [|m IH]; simpl.
-  { by constructor. }
-  intros ?. constructor; [|by apply IH]. rewrite Z.land_ones by lia.
-  apply Z.mod_pos_bound. apply Z.pow_pos_nonneg; lia.
-Qed.
-
-Lemma Z_of_little_bound n bs:
-  0 ≤ n →
-  Forall (λ b, 0 ≤ b < 2 ^ n) bs →
-  0 ≤ Z_of_little n bs < 2 ^ ((length bs) * n).
-Proof.
-  intros ? Hall.
-  induction Hall as [|b bs Hb ? IH]; [done|]; simpl.
-  apply Z_bounded_iff_bits_nonneg'; [ nia | |].
-  - apply Z.lor_nonneg. split; [|lia]. apply Z.shiftl_nonneg. lia.
-  - intros l ?. rewrite Z.lor_spec.
-    eapply Z_bounded_iff_bits_nonneg' in Hb.
-    + erewrite Hb, orb_false_r.
-      rewrite Z.shiftl_spec by nia.
-      eapply Z_bounded_iff_bits_nonneg'; [| | done |]; nia.
-    + lia.
-    + lia.
-    + nia.
-Qed.
-
-Lemma Z_to_little_length m n z : length (Z_to_little m n z) = m.
-Proof. revert z. induction m; naive_solver. Qed.
-
 (** * Preliminary definitions *)
 Definition bv_modulus (n : N) : Z := 2 ^ (Z.of_N n).
 Definition bv_half_modulus (n : N) : Z := bv_modulus n `div` 2.
@@ -316,25 +188,25 @@ Proof.
   intros. subst. f_equal. apply proof_irrel.
 Qed.
 
-Definition bv_of_Z_checked (n : N) (z : Z) : option (bv n) :=
+Definition Z_to_bv_checked (n : N) (z : Z) : option (bv n) :=
   guard (bv_wf n z) as H; Some (BV n z H).
 
-Program Definition bv_of_Z (n : N) (z : Z) : bv n :=
+Program Definition Z_to_bv (n : N) (z : Z) : bv n :=
   BV n (bv_wrap n z) _.
 Next Obligation. apply bv_wrap_wf. Qed.
 
-Lemma bv_of_Z_unsigned n z:
-  bv_unsigned (bv_of_Z n z) = bv_wrap n z.
+Lemma Z_to_bv_unsigned n z:
+  bv_unsigned (Z_to_bv n z) = bv_wrap n z.
 Proof. done. Qed.
 
-Lemma bv_of_Z_signed n z:
-  bv_signed (bv_of_Z n z) = bv_swrap n z.
+Lemma Z_to_bv_signed n z:
+  bv_signed (Z_to_bv n z) = bv_swrap n z.
 Proof. apply bv_swrap_wrap. Qed.
 
-Lemma bv_of_Z_small n z:
+Lemma Z_to_bv_small n z:
   0 ≤ z < bv_modulus n →
-  bv_unsigned (bv_of_Z n z) = z.
-Proof. rewrite bv_of_Z_unsigned. apply bv_wrap_small. Qed.
+  bv_unsigned (Z_to_bv n z) = z.
+Proof. rewrite Z_to_bv_unsigned. apply bv_wrap_small. Qed.
 
 Lemma bv_unsigned_in_range n (b : bv n):
   0 ≤ bv_unsigned b < bv_modulus n.
@@ -354,10 +226,10 @@ Qed.
 Lemma bv_signed_N_0 (b : bv 0):
   bv_signed b = 0.
 Proof. unfold bv_signed. by rewrite bv_unsigned_N_0, bv_swrap_0. Qed.
-Lemma bv_of_Z_checked_bv_unsigned n (b : bv n):
-  bv_of_Z_checked n (bv_unsigned b) = Some b.
+Lemma Z_to_bv_checked_bv_unsigned n (b : bv n):
+  Z_to_bv_checked n (bv_unsigned b) = Some b.
 Proof.
-  unfold bv_of_Z_checked. case_option_guard.
+  unfold Z_to_bv_checked. case_option_guard.
   - f_equal. by apply bv_eq.
   - by pose proof bv_is_wf b.
 Qed.
@@ -368,27 +240,27 @@ Global Program Instance bv_eq_dec n : EqDecision (bv n) := λ '(BV _ v1 p1) '(BV
    | left eqv => left _
    | right eqv => right _
    end.
-Next Obligation. intros. subst. rewrite (proof_irrel p1 p2). exact eq_refl. Defined.
+Next Obligation.  intros n b1 v1 p1 ? b2 v2 p2 ????. subst. rewrite (proof_irrel p1 p2). exact eq_refl. Defined.
 Next Obligation. intros. by injection. Qed.
 
 Global Instance bv_countable n : Countable (bv n) :=
-  inj_countable bv_unsigned (bv_of_Z_checked n) (bv_of_Z_checked_bv_unsigned n).
+  inj_countable bv_unsigned (Z_to_bv_checked n) (Z_to_bv_checked_bv_unsigned n).
 
 Global Program Instance bv_finite n : Finite (bv n) :=
-  {| enum := bv_of_Z n <$> (seqZ 0 (bv_modulus n)) |}.
+  {| enum := Z_to_bv n <$> (seqZ 0 (bv_modulus n)) |}.
 Next Obligation.
   intros n. apply NoDup_alt. intros i j x.
   rewrite !list_lookup_fmap.
   intros [? [[??]%lookup_seqZ ?]]%fmap_Some.
   intros [? [[??]%lookup_seqZ Hz]]%fmap_Some. subst.
-  apply bv_eq in Hz. rewrite !bv_of_Z_small in Hz; lia.
+  apply bv_eq in Hz. rewrite !Z_to_bv_small in Hz; lia.
 Qed.
 Next Obligation.
-  intros. apply elem_of_list_lookup. eexists (Z.to_nat (bv_unsigned x)).
+  intros n x. apply elem_of_list_lookup. eexists (Z.to_nat (bv_unsigned x)).
   rewrite list_lookup_fmap. apply fmap_Some. eexists _.
   pose proof (bv_unsigned_in_range _ x). split.
   - apply lookup_seqZ. split; [done|]. rewrite Z2Nat.id; lia.
-  - apply bv_eq. rewrite bv_of_Z_small; rewrite Z2Nat.id; lia.
+  - apply bv_eq. rewrite Z_to_bv_small; rewrite Z2Nat.id; lia.
 Qed.
 
 
@@ -411,6 +283,7 @@ Ltac bv_saturate :=
      learn_hyp (bv_unsigned_in_range _ b) | learn_hyp (bv_signed_in_range _ b)
   ] end.
 
+(* TODO: Where to put the following automation? And how should it best be implemented? *)
 Definition bv_wrap_simplify_marker (z1 z2 : Z) : Z := z1 + z2.
 
 Lemma bv_wrap_simplify_marker_intro n z x:
@@ -456,11 +329,20 @@ Lemma bv_wrap_simplify_marker_remove_end_opp n z x m:
   bv_wrap n (bv_wrap_simplify_marker (- z * bv_modulus n) m) = x.
 Proof. intros <-. unfold bv_wrap_simplify_marker. rewrite Z.add_comm. apply bv_wrap_add_modulus. Qed.
 
-Ltac bv_wrap_simplify_cancel :=
+Lemma Zmul_assoc_comm n2 n1 n3 : n1 * n2 * n3 = n1 * n3 * n2.
+Proof. lia. Qed.
+
+Lemma Zpow_2_mul a : a ^ 2 = a * a.
+Proof. lia. Qed.
+
+Local Ltac bv_wrap_simplify_cancel :=
   apply bv_wrap_simplify_marker_intro;
   repeat first [ apply bv_wrap_simplify_marker_remove | apply bv_wrap_simplify_marker_remove_sub | apply bv_wrap_simplify_marker_move];
   first [ apply bv_wrap_simplify_marker_remove_end | apply bv_wrap_simplify_marker_remove_end_opp | apply bv_wrap_simplify_marker_move_end].
 
+(** [bv_wrap_simplify] applies for goals of the form [bv_wrap n z1 = bv_wrap n z2] and
+[bv_swrap n z1 = bv_swrap n z2] and tries to simplify them by removing any [bv_wrap]
+and [bv_swrap] inside z1 and z2. *)
 Ltac bv_wrap_simplify :=
   unfold bv_signed, bv_swrap;
   try match goal with | |- _ - _ = _ - _ => f_equal end;
@@ -505,19 +387,19 @@ Qed.
 Global Instance bv_inhabited n : Inhabited (bv n) := populate (bv_0 n).
 
 Definition bv_succ {n} (x : bv n) : bv n :=
-  bv_of_Z n (Z.succ (bv_unsigned x)).
+  Z_to_bv n (Z.succ (bv_unsigned x)).
 Definition bv_pred {n} (x : bv n) : bv n :=
-  bv_of_Z n (Z.pred (bv_unsigned x)).
+  Z_to_bv n (Z.pred (bv_unsigned x)).
 
 Definition bv_add {n} (x y : bv n) : bv n := (* SMT: bvadd *)
-  bv_of_Z n (Z.add (bv_unsigned x) (bv_unsigned y)).
+  Z_to_bv n (Z.add (bv_unsigned x) (bv_unsigned y)).
 Definition bv_sub {n} (x y : bv n) : bv n := (* SMT: bvsub *)
-  bv_of_Z n (Z.sub (bv_unsigned x) (bv_unsigned y)).
+  Z_to_bv n (Z.sub (bv_unsigned x) (bv_unsigned y)).
 Definition bv_opp {n} (x : bv n) : bv n := (* SMT: bvneg *)
-  bv_of_Z n (Z.opp (bv_unsigned x)).
+  Z_to_bv n (Z.opp (bv_unsigned x)).
 
 Definition bv_mul {n} (x y : bv n) : bv n := (* SMT: bvmul *)
-  bv_of_Z n (Z.mul (bv_unsigned x) (bv_unsigned y)).
+  Z_to_bv n (Z.mul (bv_unsigned x) (bv_unsigned y)).
 Program Definition bv_divu {n} (x y : bv n) : bv n := (* SMT: bvudiv *)
   BV n (Z.div (bv_unsigned x) (bv_unsigned y)) _.
 Next Obligation.
@@ -539,16 +421,16 @@ Next Obligation.
   apply Z.mod_le; lia.
 Qed.
 Definition bv_divs {n} (x y : bv n) : bv n :=
-  bv_of_Z n (Z.div (bv_signed x) (bv_signed y)).
+  Z_to_bv n (Z.div (bv_signed x) (bv_signed y)).
 Definition bv_quots {n} (x y : bv n) : bv n := (* SMT: bvsdiv *)
-  bv_of_Z n (Z.quot (bv_signed x) (bv_signed y)).
+  Z_to_bv n (Z.quot (bv_signed x) (bv_signed y)).
 Definition bv_mods {n} (x y : bv n) : bv n := (* SMT: bvsmod *)
-  bv_of_Z n (Z.modulo (bv_signed x) (bv_signed y)).
+  Z_to_bv n (Z.modulo (bv_signed x) (bv_signed y)).
 Definition bv_rems {n} (x y : bv n) : bv n := (* SMT: bvsrem *)
-  bv_of_Z n (Z.rem (bv_signed x) (bv_signed y)).
+  Z_to_bv n (Z.rem (bv_signed x) (bv_signed y)).
 
 Definition bv_shiftl {n} (x y : bv n) : bv n := (* SMT: bvshl *)
-  bv_of_Z n (Z.shiftl (bv_unsigned x) (bv_unsigned y)).
+  Z_to_bv n (Z.shiftl (bv_unsigned x) (bv_unsigned y)).
 Program Definition bv_shiftr {n} (x y : bv n) : bv n := (* SMT: bvlshr *)
   BV n (Z.shiftr (bv_unsigned x) (bv_unsigned y)) _.
 Next Obligation.
@@ -560,7 +442,7 @@ Next Obligation.
   apply Z.div_le_upper_bound; [ lia|]. nia.
 Qed.
 Definition bv_ashiftr {n} (x y : bv n) : bv n := (* SMT: bvashr *)
-  bv_of_Z n (Z.shiftr (bv_signed x) (bv_unsigned y)).
+  Z_to_bv n (Z.shiftr (bv_signed x) (bv_unsigned y)).
 
 Program Definition bv_or {n} (x y : bv n) : bv n := (* SMT: bvor *)
   BV n (Z.lor (bv_unsigned x) (bv_unsigned y)) _.
@@ -578,20 +460,17 @@ Next Obligation.
   intros. eapply bv_wf_bitwise_op; [ apply Z.lxor_spec | intros; eapply Z.lxor_nonneg; naive_solver | done | apply bv_is_wf..].
 Qed.
 Program Definition bv_not {n} (x : bv n) : bv n := (* SMT: bvnot *)
-  bv_of_Z n (Z.lnot (bv_unsigned x)).
+  Z_to_bv n (Z.lnot (bv_unsigned x)).
 
-Program Definition bv_ugt {n} (x y : bv n) : bool :=
-  (bv_unsigned x) >? (bv_unsigned y).
+(* [bv_zero_extends z b] extends [b] to [z] bits with 0. If [z] is
+smaller than [n], [b] is truncated. Note that [z] gives the resulting
+size instead of the number of bits to add (as SMTLIB does) to avoid a
+type-level [_ + _] *)
+Program Definition bv_zero_extend {n} (z : N) (b : bv n) : bv z := (* SMT: zero_extend *)
+  Z_to_bv z (bv_unsigned b).
 
-Program Definition bv_zero_extend {n} (z : N) (b : bv n) : bv (z + n) := (* SMT: zero_extend *)
-  BV _ (bv_unsigned b) _.
-Next Obligation.
-  intros. apply bv_wf_in_range. rewrite bv_modulus_add. bv_saturate.
-  pose proof (bv_modulus_pos z). nia.
-Qed.
-
-Program Definition bv_sign_extend {n} (z : N) (b : bv n) : bv (z + n) := (* SMT: sign_extend *)
-  bv_of_Z _ (bv_signed b).
+Program Definition bv_sign_extend {n} (z : N) (b : bv n) : bv z := (* SMT: sign_extend *)
+  Z_to_bv z (bv_signed b).
 
 (* s is start index and l is length. Note that this is different from
 extract in SMTLIB which uses [extract (inclusive upper bound)
@@ -612,7 +491,7 @@ Qed.
 Program Definition bv_concat {n1 n2} (b1 : bv n1) (b2 : bv n2) : bv (n1 + n2) := (* SMT: concat *)
   BV _ (Z.lor (bv_unsigned b1 ≪ Z.of_N n2) (bv_unsigned b2)) _.
 Next Obligation.
-  intros.
+  intros n1 n2 b1 b2.
   apply bv_wf_in_range.
   apply Z_bounded_iff_bits_nonneg'; [lia | |].
   { apply Z.lor_nonneg. bv_saturate. split; [|lia]. apply Z.shiftl_nonneg. lia. }
@@ -622,19 +501,19 @@ Next Obligation.
   - apply (Z.lt_le_trans _ (bv_modulus n2)); [lia|]. apply Z.pow_le_mono_r; lia.
 Qed.
 
-Definition bv_to_little m n (z : Z) : list (bv n) :=
-  (λ b, bv_of_Z n b) <$> Z_to_little m (Z.of_N n) z.
+Definition bv_to_little_endian m n (z : Z) : list (bv n) :=
+  (λ b, Z_to_bv n b) <$> Z_to_little_endian m (Z.of_N n) z.
 
-Definition bv_of_little n (bs : list (bv n)) : Z :=
-  Z_of_little (Z.of_N n) (bv_unsigned <$> bs).
+Definition little_endian_to_bv n (bs : list (bv n)) : Z :=
+  little_endian_to_Z (Z.of_N n) (bv_unsigned <$> bs).
 
 (** * Operations on [bv n] and Z *)
 Definition bv_add_Z {n} (x : bv n) (y : Z) : bv n :=
-  bv_of_Z n (Z.add (bv_unsigned x) y).
+  Z_to_bv n (Z.add (bv_unsigned x) y).
 Definition bv_sub_Z {n} (x : bv n) (y : Z) : bv n :=
-  bv_of_Z n (Z.sub (bv_unsigned x) y).
+  Z_to_bv n (Z.sub (bv_unsigned x) y).
 Definition bv_mul_Z {n} (x : bv n) (y : Z) : bv n :=
-  bv_of_Z n (Z.mul (bv_unsigned x) y).
+  Z_to_bv n (Z.mul (bv_unsigned x) y).
 
 Definition bv_seq {n} (x : bv n) (len : Z) : list (bv n) :=
   (bv_add_Z x) <$> seqZ 0 len.
@@ -651,42 +530,42 @@ Section unfolding.
   Proof. done. Qed.
   Lemma bv_succ_signed b :
     bv_signed (bv_succ b) = bv_swrap n (Z.succ (bv_signed b)).
-  Proof. unfold bv_succ. rewrite bv_of_Z_signed. bv_wrap_simplify_solve. Qed.
+  Proof. unfold bv_succ. rewrite Z_to_bv_signed. bv_wrap_simplify_solve. Qed.
 
   Lemma bv_pred_unsigned b :
     bv_unsigned (bv_pred b) = bv_wrap n (Z.pred (bv_unsigned b)).
   Proof. done. Qed.
   Lemma bv_pred_signed b :
     bv_signed (bv_pred b) = bv_swrap n (Z.pred (bv_signed b)).
-  Proof. unfold bv_pred. rewrite bv_of_Z_signed. bv_wrap_simplify_solve. Qed.
+  Proof. unfold bv_pred. rewrite Z_to_bv_signed. bv_wrap_simplify_solve. Qed.
 
   Lemma bv_add_unsigned b1 b2 :
     bv_unsigned (bv_add b1 b2) = bv_wrap n (bv_unsigned b1 + bv_unsigned b2).
   Proof. done. Qed.
   Lemma bv_add_signed b1 b2 :
     bv_signed (bv_add b1 b2) = bv_swrap n (bv_signed b1 + bv_signed b2).
-  Proof. unfold bv_add. rewrite bv_of_Z_signed. bv_wrap_simplify_solve. Qed.
+  Proof. unfold bv_add. rewrite Z_to_bv_signed. bv_wrap_simplify_solve. Qed.
 
   Lemma bv_sub_unsigned b1 b2 :
     bv_unsigned (bv_sub b1 b2) = bv_wrap n (bv_unsigned b1 - bv_unsigned b2).
   Proof. done. Qed.
   Lemma bv_sub_signed b1 b2 :
     bv_signed (bv_sub b1 b2) = bv_swrap n (bv_signed b1 - bv_signed b2).
-  Proof. unfold bv_sub. rewrite bv_of_Z_signed. bv_wrap_simplify_solve. Qed.
+  Proof. unfold bv_sub. rewrite Z_to_bv_signed. bv_wrap_simplify_solve. Qed.
 
   Lemma bv_opp_unsigned b :
     bv_unsigned (bv_opp b) = bv_wrap n (- bv_unsigned b).
   Proof. done. Qed.
   Lemma bv_opp_signed b :
     bv_signed (bv_opp b) = bv_swrap n (- bv_signed b).
-  Proof. unfold bv_opp. rewrite bv_of_Z_signed. bv_wrap_simplify_solve. Qed.
+  Proof. unfold bv_opp. rewrite Z_to_bv_signed. bv_wrap_simplify_solve. Qed.
 
   Lemma bv_mul_unsigned b1 b2 :
     bv_unsigned (bv_mul b1 b2) = bv_wrap n (bv_unsigned b1 * bv_unsigned b2).
   Proof. done. Qed.
   Lemma bv_mul_signed b1 b2 :
     bv_signed (bv_mul b1 b2) = bv_swrap n (bv_signed b1 * bv_signed b2).
-  Proof. unfold bv_mul. rewrite bv_of_Z_signed. bv_wrap_simplify_solve. Qed.
+  Proof. unfold bv_mul. rewrite Z_to_bv_signed. bv_wrap_simplify_solve. Qed.
 
   Lemma bv_divu_unsigned b1 b2 :
     bv_unsigned (bv_divu b1 b2) = Z.div (bv_unsigned b1) (bv_unsigned b2).
@@ -707,35 +586,35 @@ Section unfolding.
   Proof. done. Qed.
   Lemma bv_divs_signed b1 b2 :
     bv_signed (bv_divs b1 b2) = bv_swrap n (Z.div (bv_signed b1) (bv_signed b2)).
-  Proof. unfold bv_divs. rewrite bv_of_Z_signed. done. Qed.
+  Proof. unfold bv_divs. rewrite Z_to_bv_signed. done. Qed.
 
   Lemma bv_quots_unsigned b1 b2 :
     bv_unsigned (bv_quots b1 b2) = bv_wrap n (Z.quot (bv_signed b1) (bv_signed b2)).
   Proof. done. Qed.
   Lemma bv_quots_signed b1 b2 :
     bv_signed (bv_quots b1 b2) = bv_swrap n (Z.quot (bv_signed b1) (bv_signed b2)).
-  Proof. unfold bv_quots. rewrite bv_of_Z_signed. done. Qed.
+  Proof. unfold bv_quots. rewrite Z_to_bv_signed. done. Qed.
 
   Lemma bv_mods_unsigned b1 b2 :
     bv_unsigned (bv_mods b1 b2) = bv_wrap n (Z.modulo (bv_signed b1) (bv_signed b2)).
   Proof. done. Qed.
   Lemma bv_mods_signed b1 b2 :
     bv_signed (bv_mods b1 b2) = bv_swrap n (Z.modulo (bv_signed b1) (bv_signed b2)).
-  Proof. unfold bv_mods. rewrite bv_of_Z_signed. done. Qed.
+  Proof. unfold bv_mods. rewrite Z_to_bv_signed. done. Qed.
 
   Lemma bv_rems_unsigned b1 b2 :
     bv_unsigned (bv_rems b1 b2) = bv_wrap n (Z.rem (bv_signed b1) (bv_signed b2)).
   Proof. done. Qed.
-  Lemma bv_rem_signed b1 b2 :
+  Lemma bv_rems_signed b1 b2 :
     bv_signed (bv_rems b1 b2) = bv_swrap n (Z.rem (bv_signed b1) (bv_signed b2)).
-  Proof. unfold bv_rems. rewrite bv_of_Z_signed. done. Qed.
+  Proof. unfold bv_rems. rewrite Z_to_bv_signed. done. Qed.
 
   Lemma bv_shiftl_unsigned b1 b2 :
     bv_unsigned (bv_shiftl b1 b2) = bv_wrap n (Z.shiftl (bv_unsigned b1) (bv_unsigned b2)).
   Proof. done. Qed.
   Lemma bv_shiftl_signed b1 b2 :
     bv_signed (bv_shiftl b1 b2) = bv_swrap n (Z.shiftl (bv_unsigned b1) (bv_unsigned b2)).
-  Proof. unfold bv_shiftl. rewrite bv_of_Z_signed. done. Qed.
+  Proof. unfold bv_shiftl. rewrite Z_to_bv_signed. done. Qed.
 
   Lemma bv_shiftr_unsigned b1 b2 :
     bv_unsigned (bv_shiftr b1 b2) = Z.shiftr (bv_unsigned b1) (bv_unsigned b2).
@@ -749,7 +628,7 @@ Section unfolding.
   Proof. done. Qed.
   Lemma bv_ashiftr_signed b1 b2 :
     bv_signed (bv_ashiftr b1 b2) = bv_swrap n (Z.shiftr (bv_signed b1) (bv_unsigned b2)).
-  Proof. unfold bv_ashiftr. rewrite bv_of_Z_signed. done. Qed.
+  Proof. unfold bv_ashiftr. rewrite Z_to_bv_signed. done. Qed.
 
   Lemma bv_or_unsigned b1 b2 :
     bv_unsigned (bv_or b1 b2) = Z.lor (bv_unsigned b1) (bv_unsigned b2).
@@ -777,48 +656,77 @@ Section unfolding.
   Proof. done. Qed.
   Lemma bv_not_signed b :
     bv_signed (bv_not b) = bv_swrap n (Z.lnot (bv_unsigned b)).
-  Proof. unfold bv_not. rewrite bv_of_Z_signed. done. Qed.
+  Proof. unfold bv_not. rewrite Z_to_bv_signed. done. Qed.
 
+  Lemma bv_zero_extend_unsigned' z b :
+    bv_unsigned (bv_zero_extend z b) = bv_wrap z (bv_unsigned b).
+  Proof. done. Qed.
+  (* [bv_zero_extend_unsigned] is the version that we want, but it
+  only holds with a precondition. *)
   Lemma bv_zero_extend_unsigned z b :
+    (n ≤ z)%N →
     bv_unsigned (bv_zero_extend z b) = bv_unsigned b.
-  Proof. done. Qed.
+  Proof.
+    intros ?. rewrite bv_zero_extend_unsigned', bv_wrap_small; [done|].
+    bv_saturate. pose proof (bv_modulus_le_mono n z). lia.
+  Qed.
   Lemma bv_zero_extend_signed z b :
-    bv_signed (bv_zero_extend z b) = bv_swrap (z + n) (bv_unsigned b).
-  Proof. done. Qed.
+    bv_signed (bv_zero_extend z b) = bv_swrap z (bv_unsigned b).
+  Proof. unfold bv_zero_extend. rewrite Z_to_bv_signed. done. Qed.
 
   Lemma bv_sign_extend_unsigned z b :
-    bv_unsigned (bv_sign_extend z b) = bv_wrap (z + n) (bv_signed b).
+    bv_unsigned (bv_sign_extend z b) = bv_wrap z (bv_signed b).
   Proof. done. Qed.
+  Lemma bv_sign_extend_signed' z b :
+    bv_signed (bv_sign_extend z b) = bv_swrap z (bv_signed b).
+  Proof. unfold bv_sign_extend. rewrite Z_to_bv_signed. done. Qed.
+  (* [bv_sign_extend_signed] is the version that we want, but it
+  only holds with a precondition. *)
   Lemma bv_sign_extend_signed z b :
+    (n ≤ z)%N →
     bv_signed (bv_sign_extend z b) = bv_signed b.
   Proof.
-    unfold bv_sign_extend. rewrite bv_of_Z_signed.
+    intros ?. rewrite bv_sign_extend_signed'.
     destruct (decide (n = 0%N)); subst.
     { by rewrite bv_signed_N_0, bv_swrap_0. }
     apply bv_swrap_small. bv_saturate.
-    pose proof bv_half_modulus_le_mono n (z + n). lia.
+    pose proof bv_half_modulus_le_mono n z. lia.
   Qed.
+
+  Lemma bv_extract_unsigned s l b :
+    bv_unsigned (bv_extract s l b) = Z.land (bv_unsigned b ≫ Z.of_N s) (Z.ones (Z.of_N l)).
+  Proof. done. Qed.
+  Lemma bv_extract_signed s l b :
+    bv_signed (bv_extract s l b) = bv_swrap l (Z.land (bv_unsigned b ≫ Z.of_N s) (Z.ones (Z.of_N l))).
+  Proof. done. Qed.
+
+  Lemma bv_concat_unsigned n2 b1 (b2 : bv n2) :
+    bv_unsigned (bv_concat b1 b2) = Z.lor (bv_unsigned b1 ≪ Z.of_N n2) (bv_unsigned b2).
+  Proof. done. Qed.
+  Lemma bv_concat_signed n2 b1 (b2 : bv n2) :
+    bv_signed (bv_concat b1 b2) = bv_swrap (n + n2) (Z.lor (bv_unsigned b1 ≪ Z.of_N n2) (bv_unsigned b2)).
+  Proof. done. Qed.
 
   Lemma bv_add_Z_unsigned b z :
     bv_unsigned (bv_add_Z b z) = bv_wrap n (bv_unsigned b + z).
   Proof. done. Qed.
   Lemma bv_add_Z_signed b z :
     bv_signed (bv_add_Z b z) = bv_swrap n (bv_signed b + z).
-  Proof. unfold bv_add_Z. rewrite bv_of_Z_signed. bv_wrap_simplify_solve. Qed.
+  Proof. unfold bv_add_Z. rewrite Z_to_bv_signed. bv_wrap_simplify_solve. Qed.
 
   Lemma bv_sub_Z_unsigned b z :
     bv_unsigned (bv_sub_Z b z) = bv_wrap n (bv_unsigned b - z).
   Proof. done. Qed.
   Lemma bv_sub_Z_signed b z :
     bv_signed (bv_sub_Z b z) = bv_swrap n (bv_signed b - z).
-  Proof. unfold bv_sub_Z. rewrite bv_of_Z_signed. bv_wrap_simplify_solve. Qed.
+  Proof. unfold bv_sub_Z. rewrite Z_to_bv_signed. bv_wrap_simplify_solve. Qed.
 
   Lemma bv_mul_Z_unsigned b z:
     bv_unsigned (bv_mul_Z b z) = bv_wrap n (bv_unsigned b * z).
   Proof. done. Qed.
   Lemma bv_mul_Z_signed b z :
     bv_signed (bv_mul_Z b z) = bv_swrap n (bv_signed b * z).
-  Proof. unfold bv_mul_Z. rewrite bv_of_Z_signed. bv_wrap_simplify_solve. Qed.
+  Proof. unfold bv_mul_Z. rewrite Z_to_bv_signed. bv_wrap_simplify_solve. Qed.
 End unfolding.
 
 (** ** Properties of bv operations *)
@@ -829,88 +737,110 @@ Section properties.
   Lemma bv_sub_add_opp b1 b2:
     bv_sub b1 b2 = bv_add b1 (bv_opp b2).
   Proof.
-    apply bv_eq. unfold bv_sub, bv_add, bv_opp. rewrite !bv_of_Z_unsigned.
+    apply bv_eq. unfold bv_sub, bv_add, bv_opp. rewrite !Z_to_bv_unsigned.
     bv_wrap_simplify_solve.
   Qed.
 
   Global Instance bv_add_assoc : Assoc (=) (@bv_add n).
   Proof.
-    intros ???. unfold bv_add. apply bv_eq. rewrite !bv_of_Z_unsigned.
+    intros ???. unfold bv_add. apply bv_eq. rewrite !Z_to_bv_unsigned.
     bv_wrap_simplify_solve.
   Qed.
 
   Global Instance bv_mul_assoc : Assoc (=) (@bv_mul n).
   Proof.
-    intros ???. unfold bv_mul. apply bv_eq. rewrite !bv_of_Z_unsigned.
+    intros ???. unfold bv_mul. apply bv_eq. rewrite !Z_to_bv_unsigned.
     bv_wrap_simplify_solve.
   Qed.
 
   Lemma bv_add_Z_0 b : bv_add_Z b 0 = b.
   Proof.
     unfold bv_add_Z. rewrite Z.add_0_r.
-    apply bv_eq. apply bv_of_Z_small. apply bv_unsigned_in_range.
+    apply bv_eq. apply Z_to_bv_small. apply bv_unsigned_in_range.
   Qed.
 
   Lemma bv_add_Z_add_r b m o:
     bv_add_Z b (m + o) = bv_add_Z (bv_add_Z b o) m.
   Proof.
-    apply bv_eq. unfold bv_add_Z. rewrite !bv_of_Z_unsigned.
+    apply bv_eq. unfold bv_add_Z. rewrite !Z_to_bv_unsigned.
      bv_wrap_simplify_solve.
   Qed.
 
   Lemma bv_add_Z_add_l b m o:
     bv_add_Z b (m + o) = bv_add_Z (bv_add_Z b m) o.
   Proof.
-    apply bv_eq. unfold bv_add_Z. rewrite !bv_of_Z_unsigned.
+    apply bv_eq. unfold bv_add_Z. rewrite !Z_to_bv_unsigned.
      bv_wrap_simplify_solve.
   Qed.
 
   Lemma bv_add_Z_succ b m:
     bv_add_Z b (Z.succ m) = bv_add_Z (bv_add_Z b 1) m.
   Proof.
-    apply bv_eq. unfold bv_add_Z. rewrite !bv_of_Z_unsigned.
-      bv_wrap_simplify_solve.
+    apply bv_eq. unfold bv_add_Z. rewrite !Z_to_bv_unsigned.
+    bv_wrap_simplify_solve.
   Qed.
 
+  Lemma bv_concat_0 m b1 (b2 : bv m) :
+    bv_unsigned b1 = 0 →
+    bv_concat b1 b2 = bv_zero_extend (n + m) b2.
+  Proof.
+    intros Hb1. apply bv_eq.
+    rewrite bv_zero_extend_unsigned; [|lia].
+    by rewrite bv_concat_unsigned, Hb1, Z.shiftl_0_l, Z.lor_0_l.
+  Qed.
 End properties.
 
 (** ** Lemmas about [bv_to_little] and [bv_of_little] *)
 Section little.
 
-  Lemma bv_to_litte_unsigned m n z:
-    bv_unsigned <$> bv_to_little m n z = Z_to_little m (Z.of_N n) z.
+  Lemma bv_to_litte_endian_unsigned m n z:
+    0 ≤ m →
+    bv_unsigned <$> bv_to_little_endian m n z = Z_to_little_endian m (Z.of_N n) z.
   Proof.
-    apply list_eq. intros i. unfold bv_to_little.
+    intros ?. apply list_eq. intros i. unfold bv_to_little_endian.
     rewrite list_lookup_fmap, list_lookup_fmap.
-    destruct (Z_to_little m (Z.of_N n) z !! i) eqn: Heq; [simpl |done].
-    rewrite bv_of_Z_small; [done|].
-    eapply (Forall_forall (λ z, _ ≤ z < _)); [ eapply Z_to_little_bound; lia | ].
-    by eapply elem_of_list_lookup_2.
+    destruct (Z_to_little_endian m (Z.of_N n) z !! i) eqn: Heq; [simpl |done].
+    rewrite Z_to_bv_small; [done|].
+    eapply (Forall_forall (λ z, _ ≤ z < _)); [ |by eapply elem_of_list_lookup_2].
+    eapply Z_to_little_endian_bound; lia.
   Qed.
 
-  Lemma bv_to_of_little m n bs:
-    m = length bs →
-    bv_to_little m n (bv_of_little n bs) = bs.
+  Lemma bv_to_little_endian_to_bv m n bs:
+    m = Z.of_nat (length bs) →
+    bv_to_little_endian m n (little_endian_to_bv n bs) = bs.
   Proof.
     intros ->. eapply (fmap_inj bv_unsigned). { intros ???. by apply bv_eq. }
-    rewrite bv_to_litte_unsigned. apply Z_to_of_little; [by rewrite fmap_length | lia |].
+    rewrite bv_to_litte_endian_unsigned; [|lia].
+    apply Z_to_little_endian_to_Z; [by rewrite fmap_length | lia |].
     apply Forall_forall. intros ? [?[->?]]%elem_of_list_fmap_2. apply bv_unsigned_in_range.
   Qed.
 
-  Lemma bv_of_to_little m n z:
-    bv_of_little n (bv_to_little m n z) = z `mod` 2 ^ (m * Z.of_N n).
-  Proof. unfold bv_of_little. rewrite bv_to_litte_unsigned. apply Z_of_to_little. lia. Qed.
+  Lemma little_endian_to_bv_to_little_endian m n z:
+    0 ≤ m →
+    little_endian_to_bv n (bv_to_little_endian m n z) = z `mod` 2 ^ (m * Z.of_N n).
+  Proof.
+    intros ?. unfold little_endian_to_bv.
+    rewrite bv_to_litte_endian_unsigned; [|lia].
+    apply little_endian_to_Z_to_little_endian; lia.
+  Qed.
 
-  Lemma bv_to_little_length m n z : length (bv_to_little m n z) = m.
-  Proof. unfold bv_to_little. rewrite fmap_length. apply Z_to_little_length. Qed.
+  Lemma bv_to_little_endian_length m n z :
+    0 ≤ m →
+    length (bv_to_little_endian m n z) = Z.to_nat m.
+  Proof.
+    intros ?. unfold bv_to_little_endian. rewrite fmap_length.
+    apply Nat2Z.inj. rewrite Z_to_little_endian_length, ?Z2Nat.id; try lia.
+  Qed.
 
   Lemma bv_of_to_little_bv x m n (b : bv x):
-    x = (N.of_nat m * n)%N →
-    bv_of_Z x (bv_of_little n (bv_to_little m n (bv_unsigned b))) = b.
+    0 ≤ m →
+    x = (Z.to_N m * n)%N →
+    Z_to_bv x (little_endian_to_bv n (bv_to_little_endian m n (bv_unsigned b))) = b.
   Proof.
-    intros ->. rewrite bv_of_to_little, Z.mod_small.
-    2: { pose proof bv_unsigned_in_range _ b. unfold bv_modulus in *. lia. }
-     apply bv_eq. rewrite bv_of_Z_small; [done|]. apply bv_unsigned_in_range.
+    intros ? ->. rewrite little_endian_to_bv_to_little_endian, Z.mod_small; [| |lia].
+    - apply bv_eq. rewrite Z_to_bv_small; [done|]. apply bv_unsigned_in_range.
+    - pose proof bv_unsigned_in_range _ b as Hr. unfold bv_modulus in Hr.
+      by rewrite N2Z.inj_mul, Z2N.id in Hr.
   Qed.
 End little.
 
@@ -932,73 +862,6 @@ Section bv_seq.
   Qed.
 End bv_seq.
 
-Section bv_zero_extend.
-  Context {n m l : N}.
-  Implicit Types (b : bv n).
-
-
-  Lemma bv_concat_zero_extend b (b1 : bv m) : bv_unsigned b1 = 0 → bv_concat b1 b = bv_zero_extend m b. 
-  Proof.
-    intros z.
-    apply bv_eq.
-    unfold bv_concat, bv_zero_extend.
-    unfold bv_unsigned at 1.
-    unfold bv_unsigned at 3.
-    rewrite z.
-    rewrite Z.shiftl_0_l.
-    by rewrite Z.lor_0_l.
-  Qed.
-  
-  Lemma bv_zero_extend_compose b : bv_unsigned (bv_zero_extend l (bv_zero_extend m b)) = bv_unsigned (bv_zero_extend (l + m) b).
-  Proof.
-    f_equal.
-  Qed.
-End bv_zero_extend.
-
-Section topbits.
-  Definition top_bits_mask (n m : Z) : Z := Z.shiftl (n-m) (Z.ones m). 
-  Definition top_bits {n} m (b : bv n) := bv_and b (bv_of_Z n (top_bits_mask (Z.of_N n) (Z.of_N m))).
-  Definition top_bits_zero {n} m (b : bv n) := bv_unsigned (top_bits m b) = 0.
-End topbits.
-
-Section unproven.
-  (* Some useful lemmas I believe to be true but haven't had time to prove *)
-  Lemma top_bits_zero_lt {n} m (b : bv n) : (top_bits_zero m b) ↔ (bv_unsigned b <  bv_modulus (n - m)).
-  Admitted.
-
-  Lemma extract_non_zero_bits {n} m (b : bv n) (H : top_bits_zero (n - m) b) : bv_unsigned (bv_extract 0 m b) = bv_unsigned b.
-  Admitted.
-
-  Lemma bv_ugt_unsigned {n} (b b' : bv n) : bv_ugt b b' = true ↔ bv_unsigned b > bv_unsigned b'.
-  Admitted.
-End unproven.
-
-(* Some automation for discharging a subset of bv goals that are equivalent to integer goals that can be handled by lia *)
-(* This is currently all very ad hoc *)
-
-Ltac erase_top_bits :=
-  (match goal with 
-  | Q:top_bits_zero _ _ |- _ => apply top_bits_zero_lt in Q
-  end).
-
-Ltac bv_simplify_step :=
-  match goal with
-  | |- context [bv_concat ?b] => rewrite bv_concat_zero_extend; [|done]
-  (* This used to match [@eq (bv _)], but that stops it matching addr which is [bv 64], this seems to work *)
-  | |- (?b1 = _) => match type of b1 with (bv _) => apply bv_eq end
-  | |- context [bv_unsigned (@bv_zero_extend ?n ?z _)] => rewrite (@bv_zero_extend_unsigned n z)
-  | |- context [bv_unsigned (bv_extract _ _ _)] => rewrite extract_non_zero_bits; [|apply top_bits_zero_lt; erase_top_bits; bv_solve]
-  | |- context [bv_unsigned (bv_add _ _ )] => rewrite bv_add_unsigned
-  | |- context [bv_unsigned (bv_sub _ _ )] => rewrite bv_sub_unsigned
-  | Q : bv_ugt _ _ = true |- _ => apply bv_ugt_unsigned in Q (* apply not rewrite because this seems to hit an obscure ssreflect bug *)
-  end
-with bv_solve :=
-  repeat bv_simplify_step;
-  repeat unfold bv_modulus, bv_wrap, bv_unsigned in *;
-  repeat (match goal with Q:bv _ |- _ => destruct Q end);
-  simpl in *;
-  lia.
-  
 (** * [bvn] *)
 Record bvn := BVN {
   bvn_n : N;
@@ -1042,116 +905,3 @@ Goal ([BV{2} 3 ] =@{bvn} [BV{10} 5]). Abort.
 Fail Goal ([BV{2} 4 ] = [BV{2} 5]).
 Goal bvn_to_bv 2 [BV{2} 3] = Some [BV{2} 3]. done. Abort.
 End test.
-
-
-
-Section test_automation.
-  Context (n : N).
-  Implicit Type a : bv n.
-  Goal ∀ a n1 n2,
-      bv_of_Z n (bv_unsigned (bv_of_Z n (bv_unsigned a + n1)) + n2) =
-      bv_of_Z n (bv_unsigned a + (n1 + n2)).
-    intros ???.
-    apply bv_eq. rewrite !bv_of_Z_unsigned. bv_wrap_simplify_solve.
-    all: fail.
-  Abort.
-
-  Goal ∀ a n1 n2,
-      bv_of_Z n (bv_unsigned (bv_of_Z n (bv_unsigned a + n1 * n1)) + bv_unsigned (bv_of_Z n n2)) =
-      bv_of_Z n (bv_unsigned a + (n1 * bv_unsigned (bv_of_Z n n1) + n2)).
-    intros ???.
-    apply bv_eq. rewrite !bv_of_Z_unsigned. bv_wrap_simplify_solve.
-    all: fail.
-  Abort.
-End test_automation.
-
-(*
-(*** Work in progress benchmarks for the automation  *)
-(* TODO: Coq.micromega.ZifyClasses does not yet exist in Coq 8.10.2 *)
-Require Import Coq.micromega.ZifyClasses.
-
-Global Instance Inj_bv_Z n : InjTyp (bv n) Z :=
-  mkinj _ _ bv_unsigned (fun x => 0 ≤ x < bv_modulus n ) (bv_unsigned_in_range _).
-
-Global Instance Op_bv_unsigned n : UnOp bv_unsigned :=
-  { TUOp := fun x => x ; TUOpInj := (fun x : bv n => @eq_refl Z (bv_unsigned x)) }.
-
-Global Instance Op_bv_eq n : BinRel (@eq (bv n)) :=
-  {| TR := @eq Z ; TRInj := bv_eq n |}.
-
-Section test_automation.
-  Context (n : N).
-  Implicit Type a : bv n.
-  Implicit Type l : list nat.
-
-  Add InjTyp (Inj_bv_Z n).
-  Add UnOp (Op_bv_unsigned n).
-  Add BinRel (Op_bv_eq n).
-
-  Goal ∀ a n1 n2,
-      bv_of_Z n (bv_unsigned (bv_of_Z n (bv_unsigned a + n1)) + n2) =
-      bv_of_Z n (bv_unsigned a + (n1 + n2)).
-  Abort.
-
-
-  Goal ∀ a z, 0 ≤ bv_unsigned a < bv_modulus n * bv_modulus z.
-    intros. pose proof (bv_modulus_pos z). nia.
-  Abort.
-
-  (* Goal ∀ a, a = a. *)
-  (*   zify. *)
-  (* Goal ∀ a, bv_of_Z n (bv_unsigned a + 0) = a. *)
-  (*   zify. *)
-  (*   bv_of_Z n (bv_unsigned a) = a *)
-  (* Abort. *)
-
-  Goal ∀ a1 a2,
-      bv_unsigned a2 ≤ bv_unsigned a1 →
-      a1 ≠ a2 → Z.to_nat (bv_unsigned a1 - bv_unsigned a2) ≠ 0%nat.
-    intros ???. rewrite bv_eq. lia.
-  Abort.
-
-  Goal ∀ a a0 m, bv_of_Z n (bv_unsigned a + m) = bv_of_Z n (bv_unsigned a0 + m) → a = a0.
-  Abort.
-
-  Goal ∀ a m n', bv_of_Z n (bv_unsigned a + m) = bv_of_Z n (bv_unsigned a + n') → m = n'.
-  Abort.
-
-  Goal ∀ a1 a2 l,
-      bv_unsigned a1 ≤ bv_unsigned a2 ∧ bv_unsigned a2 < bv_unsigned a1 + S (length l) →
-      a2 ≠ a1 →
-      bv_unsigned (bv_succ a1) ≤ bv_unsigned a2 ∧ bv_unsigned a2 < bv_unsigned (bv_succ a1) + length l.
-  Abort.
-
-  Goal ∀ a2 l,
-      bv_unsigned a2 + S (length l) < bv_modulus n →
-      bv_unsigned (bv_succ a2) + length l < bv_modulus n.
-  Abort.
-
-  Goal ∀ a1 a2 l,
-      bv_unsigned a2 + S (length l) < bv_modulus n →
-      bv_unsigned a1 < bv_unsigned a2 ∨ bv_unsigned a2 + S (length l) ≤ bv_unsigned a1→
-      bv_unsigned a1 < bv_unsigned (bv_succ a2) ∨ bv_unsigned (bv_succ a2) + length l ≤ bv_unsigned a1.
-  Abort.
-
-  Goal ∀ a1 a2 l,
-      bv_unsigned a1 < bv_unsigned a2 ∨ bv_unsigned a2 + S (length l) ≤ bv_unsigned a1 →
-      a2 ≠ a1.
-  Abort.
-
-  Goal ∀ a1 a2 l,
-      bv_unsigned a2 + S (length l) < bv_modulus n →
-      a1 ≠ a2 →
-      bv_unsigned a2 ≤ bv_unsigned a1 ∧ bv_unsigned a1 < bv_unsigned a2 + S (length l) →
-      bv_unsigned (bv_succ a2) ≤ bv_unsigned a1 ∧ bv_unsigned a1 < bv_unsigned (bv_succ a2) + length l.
-  Abort.
-
-  Goal ∀ a1 a2 l,
-      bv_unsigned a2 + S (length l) < bv_modulus n →
-      bv_unsigned a2 ≤ bv_unsigned a1 ∧ bv_unsigned a1 < bv_unsigned a2 + S (length l) →
-      a1 ≠ a2 →
-      Z.to_nat (bv_unsigned a1 - bv_unsigned (bv_succ a2)) =
-      Init.Nat.pred (Z.to_nat (bv_unsigned a1 - bv_unsigned a2)).
-  Abort.
-End test_automation.
-*)
