theories/base.v
@@ -3,7 +3,6 @@ Declare ML Module "gc_plugin".
 From Coq Require Export ssreflect.
 From stdpp Require Export prelude strings gmap.
 From RecordUpdate Require Export RecordSet.
-From refframe Require Export module.
 From refinedc.lang Require Export base.
 Require Export isla.bitvector.
 Export RecordSetNotations.
@@ -19,17 +18,10 @@ Arguments set _ _ _ _ _ !_ /.
 
 Arguments N.mul : simpl never.
 
-(* TODO: add this to the bitvector library? *)
-Global Opaque bv_eq_dec bvn_eq_dec
-       bv_0 bv_succ bv_pred
-       bv_add bv_sub bv_opp
-       bv_mul bv_divu bv_modu
-       bv_divs bv_quots bv_mods bv_rems
-       bv_shiftl bv_shiftr bv_ashiftr bv_or
-       bv_and bv_xor bv_not bv_zero_extend
-       bv_sign_extend bv_extract bv_concat
-       bv_add_Z bv_sub_Z bv_mul_Z.
-
+Ltac unLET :=
+  repeat match goal with
+         | H := _ |- _ => unfold H in *; clear H
+         end.
 
 (* This has as better performance characteristic wrt. simpl compared
 to list_find since list_find_idx does not contain prod_map. *)
