theories/bitvector_auto.v
@@ -1,0 +1,74 @@
+From isla Require Export base.
+
+Global Opaque Z_to_bv
+       bv_0 bv_succ bv_pred
+       bv_add bv_sub bv_opp
+       bv_mul bv_divu bv_modu
+       bv_divs bv_quots bv_mods bv_rems
+       bv_shiftl bv_shiftr bv_ashiftr bv_or
+       bv_and bv_xor bv_not bv_zero_extend
+       bv_sign_extend bv_extract bv_concat
+       bv_add_Z bv_sub_Z bv_mul_Z.
+
+(** The [bv_simplify] database collects rewrite rules that rewrite
+bitvectors into other bitvectors. *)
+Create HintDb bv_simplify discriminated.
+Hint Rewrite @bv_concat_0 using done : bv_simplify.
+
+(** The [bv_unfold] database contains rewrite rules that propagate
+bv_unsigned and bv_signed and unfold the bitvector definitions. *)
+Create HintDb bv_unfold discriminated.
+Lemma bv_unsigned_BV n z Heq:
+  bv_unsigned (BV n z Heq) = z.
+Proof. done. Qed.
+
+(* Rules without sideconditions *)
+Hint Rewrite
+     @bv_succ_unsigned @bv_succ_signed
+     @bv_pred_unsigned @bv_pred_signed
+     @bv_add_unsigned @bv_add_signed
+     @bv_sub_unsigned @bv_sub_signed
+     @bv_opp_unsigned @bv_opp_signed
+     @bv_mul_unsigned @bv_mul_signed
+     @bv_divu_unsigned @bv_divu_signed
+     @bv_modu_unsigned @bv_modu_signed
+     @bv_divs_unsigned @bv_divs_signed
+     @bv_quots_unsigned @bv_quots_signed
+     @bv_mods_unsigned @bv_mods_signed
+     @bv_rems_unsigned @bv_rems_signed
+     @bv_shiftl_unsigned @bv_shiftl_signed
+     @bv_shiftr_unsigned @bv_shiftr_signed
+     @bv_ashiftr_unsigned @bv_ashiftr_signed
+     @bv_or_unsigned @bv_or_signed
+     @bv_and_unsigned @bv_and_signed
+     @bv_xor_unsigned @bv_xor_signed
+     @bv_not_unsigned @bv_not_signed
+     @bv_zero_extend_signed
+     @bv_sign_extend_unsigned
+     @bv_extract_unsigned @bv_extract_signed
+     @bv_add_Z_unsigned @bv_add_Z_signed
+     @bv_sub_Z_unsigned @bv_sub_Z_signed
+     @bv_mul_Z_unsigned @bv_mul_Z_signed
+     @bv_unsigned_BV
+  : bv_unfold.
+
+(* Rules with sideconditions *)
+Hint Rewrite
+     @bv_zero_extend_unsigned @bv_sign_extend_signed
+     using lia
+  : bv_unfold.
+
+(** The [bv_unfolded_simplify] database collects rewrite rules that
+should be used to simplify the goal after Z is bv_unfolded. *)
+Create HintDb bv_unfolded_simplify discriminated.
+Hint Rewrite Z.shiftr_0_r : bv_unfolded_simplify.
+Hint Rewrite Z.land_ones using lia : bv_unfolded_simplify.
+
+Ltac bv_solve :=
+  unLET;
+  autorewrite with bv_simplify;
+  apply bv_eq;
+  autorewrite with bv_unfold;
+  autorewrite with bv_unfolded_simplify;
+  unfold bv_wrap, bv_modulus, bv_unsigned in *;
+  lia.
